examples/machine-code/instruction-set-models/x86/x86_Script.sml
@@ -2,7 +2,8 @@
 open HolKernel boolLib bossLib Parse;
 open wordsTheory bit_listTheory;
 
-open x86_coretypesTheory x86_astTheory x86_opsemTheory x86_seq_monadTheory x86_decoderTheory ;
+open x86_coretypesTheory x86_astTheory x86_opsemTheory; 
+open x86_seq_monadTheory x86_decoderTheory x86_icacheTheory;
 
 val _ = new_theory "x86_";
 
@@ -23,26 +24,29 @@ val x86_execute_some_def = Define `
 
 val X86_NEXT_def = Define `
   X86_NEXT s = 
-    let e = XREAD_EIP s in                                   (* read eip *)
-    let xs = MAP THE (XREAD_MEM_BYTES 20 e s) in             (* read next 20 bytes *)
-    let m = x86_decode_bytes xs in                           (* attempt to decode *)
-      if m = NONE then NONE else                             (* if decoded fail, return NONE *)
-        let (i,w) = THE m in                                 (* otherwise extract content *)
-        let n = 20 - (LENGTH w DIV 8) in                     (* calc length of instruction *)
-          if EVERY (\x. ~(x = NONE)) (XREAD_MEM_BYTES n e s) (* check that the memory is there *)
-          then x86_execute_some i (n2w n) s else NONE        (* execute the instruction *)`; 
+    let e = XREAD_EIP s in                                     (* read eip *)
+    let xs = MAP THE (XREAD_INSTR_BYTES 20 e s) in             (* read next 20 bytes *)
+    let m = x86_decode_bytes xs in                             (* attempt to decode *)
+      if m = NONE then NONE else                               (* if decoded fail, return NONE *)
+        let (i,w) = THE m in                                   (* otherwise extract content *)
+        let n = 20 - (LENGTH w DIV 8) in                       (* calc length of instruction *)
+          if EVERY (\x. ~(x = NONE)) (XREAD_INSTR_BYTES n e s) (* check that the memory is there *)
+          then x86_execute_some i (n2w n) s else NONE          (* execute the instruction *)`; 
+
+val X86_NEXT_REL_def = Define `
+  X86_NEXT_REL s t = ?u. X86_ICACHE s u /\ (X86_NEXT u = SOME t)`;
 
 
 (* help to evaluate X86_NEXT *)
 
 val X86_NEXT_THM = store_thm("X86_NEXT_THM",
   ``(x86_decode xs = SOME (i,w)) ==>
-    (FOLDR APPEND [] (MAP w2bits (MAP THE (XREAD_MEM_BYTES 20 (XREAD_EIP s) s))) = xs) ==>
-    (EVERY (\x. ~(x = NONE)) (XREAD_MEM_BYTES (20 - (LENGTH w DIV 8)) (XREAD_EIP s) s)) ==>
+    (FOLDR APPEND [] (MAP w2bits (MAP THE (XREAD_INSTR_BYTES 20 (XREAD_EIP s) s))) = xs) ==>
+    (EVERY (\x. ~(x = NONE)) (XREAD_INSTR_BYTES (20 - (LENGTH w DIV 8)) (XREAD_EIP s) s)) ==>
     (x86_execute iiid_dummy i (n2w (20 - (LENGTH w DIV 8))) s = SOME (tt,s')) ==>
     (X86_NEXT s = SOME s')``,
   SIMP_TAC std_ss [X86_NEXT_def,LET_DEF,XREAD_REG_def,x86_decode_bytes_def,
     x86_execute_some_def,option_apply_def]);
 
-
+  
 val _ = export_theory ();
