examples/machine-code/lisp/lisp_finalScript.sml
@@ -1,0 +1,585 @@
+open HolKernel boolLib bossLib Parse; val _ = new_theory "lisp_final";
+
+open lisp_evalTheory lisp_parseTheory lisp_printTheory lisp_proofTheory;
+open lisp_invTheory;
+open pairSyntax helperLib;
+open listTheory pred_setTheory;
+open progTheory addressTheory set_sepTheory;
+open finite_mapTheory;
+
+val aLISP_def = lisp_opsTheory.aLISP_def;
+val pLISP_def = lisp_opsTheory.pLISP_def;
+val xLISP_def = lisp_opsTheory.xLISP_def;
+
+(* aid in hiding the code, temporarily *)
+
+fun take_until p [] = []
+  | take_until p (x::xs) = if p x then [] else x:: take_until p xs 
+
+val code_abbreviations = ref ([]:thm list);
+fun add_code_abbrev thms = (code_abbreviations := thms @ !code_abbreviations);
+
+fun ABBREV_CODE_RULE name th = let
+  val (m,_,c,_) = (dest_spec o concl o SPEC_ALL) th
+  val model_name = (to_lower o implode o take_until (fn x => x = #"_") o explode o fst o dest_const) m
+  val x = list_mk_pair (free_vars c)
+  val def_name = name ^ "_" ^ model_name
+  val v = mk_var(def_name,type_of(mk_pabs(x,c)))
+  val code_def = new_definition(def_name ^ "_def",mk_eq(mk_comb(v,x),c))
+  val th = CONV_RULE ((RATOR_CONV o RAND_CONV) 
+           (ONCE_REWRITE_CONV [GSYM code_def])) (UNDISCH_ALL th)
+  val _ = add_code_abbrev [code_def]
+  in th end;
+
+(* SPEC tools *)
+
+fun SPEC_STRENGTHEN_RULE th pre = let
+  val th = SPEC pre (MATCH_MP progTheory.SPEC_STRENGTHEN th)
+  val goal = (fst o dest_imp o concl) th
+  in (th,goal) end;
+  
+fun SPEC_WEAKEN_RULE th post = let
+  val th = SPEC post (MATCH_MP progTheory.SPEC_WEAKEN th)
+  val goal = (fst o dest_imp o concl) th
+  in (th,goal) end;
+
+fun SPEC_FRAME_RULE th frame = 
+  SPEC frame (MATCH_MP progTheory.SPEC_FRAME th)
+
+fun SPEC_BOOL_FRAME_RULE th frame = let
+  val th = MATCH_MP progTheory.SPEC_FRAME th
+  val th = Q.SPEC `cond boolean_variable_name` th
+  val th = INST [mk_var("boolean_variable_name",``:bool``) |-> frame] th
+  in th end
+
+fun subst_SPEC_PC th tm = let
+  val p = find_term (can (match_term ``aPC p``)) (cdr (concl th)) handle e =>
+          find_term (can (match_term ``pPC p``)) (cdr (concl th)) handle e =>
+          find_term (can (match_term ``xPC p``)) (cdr (concl th))
+  val p = cdr p
+  val tm = subst [mk_var("p",``:word32``) |-> p] tm
+  in tm end;
+
+fun spec_pre th = let
+  val (_,p,_,_) = dest_spec (concl th) in (list_dest dest_star p, type_of p) end;
+fun spec_post th = let
+  val (_,_,_,q) = dest_spec (concl th) in (list_dest dest_star q, type_of q) end;
+
+fun spec_post_and_pre th1 th2 = let
+  val (_,_,_,q) = dest_spec (concl th1)
+  val (_,p,_,_) = dest_spec (concl th2)
+  in (list_dest dest_star q, list_dest dest_star p, type_of q) end;
+
+fun DISCH_ALL_AS_SINGLE_IMP th = let
+  val th = RW [AND_IMP_INTRO] (DISCH_ALL th)
+  in if is_imp (concl th) then th else DISCH ``T`` th end
+
+fun remove_primes th = let
+  fun last s = substring(s,size s-1,1)
+  fun delete_last_prime s = if last s = "'" then substring(s,0,size(s)-1) else hd []
+  fun foo [] ys i = i
+    | foo (x::xs) ys i = let 
+      val name = (fst o dest_var) x 
+      val new_name = repeat delete_last_prime name
+      in if name = new_name then foo xs (x::ys) i else let 
+        val new_var = mk_var(new_name,type_of x)
+        in foo xs (new_var::ys) ((x |-> new_var) :: i) end end
+  val i = foo (free_varsl (concl th :: hyp th)) [] []
+  in INST i th end
+
+fun find_composition1 th1 th2 = let
+  val (q,p,ty) = spec_post_and_pre th1 th2
+  fun get_match_term tm = get_sep_domain tm
+  fun mm x y = get_match_term x = get_match_term y
+  fun fetch_match x [] zs = hd []
+    | fetch_match x (y::ys) zs = 
+        if mm x y then (y, rev zs @ ys) else fetch_match x ys (y::zs)
+  fun partition [] ys (xs1,xs2,ys1) = (rev xs1, rev xs2, rev ys1, ys)
+    | partition (x::xs) ys (xs1,xs2,ys1) =
+        let val (y,zs) = fetch_match x ys [] in
+          partition xs zs (x::xs1, xs2, y::ys1)
+        end handle e =>
+          partition xs ys (xs1, x::xs2, ys1)
+  val (xs1,xs2,ys1,ys2) = partition q p ([],[],[])
+  val tm1 = mk_star (list_mk_star xs1 ty, list_mk_star xs2 ty)
+  val tm2 = mk_star (list_mk_star ys1 ty, list_mk_star ys2 ty)
+  val th1 = CONV_RULE (POST_CONV (MOVE_STAR_CONV tm1)) th1    
+  val th2 = CONV_RULE (PRE_CONV (MOVE_STAR_CONV tm2)) th2 
+  val th = MATCH_MP SPEC_FRAME_COMPOSE (DISCH_ALL_AS_SINGLE_IMP th2)   
+  val th = MATCH_MP th (DISCH_ALL_AS_SINGLE_IMP th1)   
+  val th = UNDISCH_ALL (PURE_REWRITE_RULE [GSYM AND_IMP_INTRO,AND_CLAUSES] th)
+  val th = SIMP_RULE std_ss [INSERT_UNION_EQ,UNION_EMPTY,word_arith_lemma1,
+             word_arith_lemma2,word_arith_lemma3,word_arith_lemma4,SEP_CLAUSES] th
+  in remove_primes th end;
+
+fun find_composition2 th1 th2 = let
+  val (q,p,ty) = spec_post_and_pre th1 th2
+  val post_not_hidden = map get_sep_domain (filter (not o can dest_sep_hide) q)
+  val pre_not_hidden  = map get_sep_domain (filter (not o can dest_sep_hide) p)
+  fun f (d:term,(zs,to_be_hidden)) = 
+    if not (can dest_sep_hide d) then (zs,to_be_hidden) else
+      (zs,filter (fn x => get_sep_domain d = x) zs @ to_be_hidden)
+  val hide_from_post = snd (foldr f (post_not_hidden,[]) p) 
+  val hide_from_pre  = snd (foldr f (pre_not_hidden,[]) q) 
+  val th1 = foldr (uncurry HIDE_POST_RULE) th1 hide_from_post
+  val th2 = foldr (uncurry HIDE_PRE_RULE) th2 hide_from_pre
+  in find_composition1 th1 th2 end;
+
+val SPEC_COMPOSE_RULE = find_composition2;    
+
+fun LISP_SPEC_COMPOSE_RULE [] = hd []
+  | LISP_SPEC_COMPOSE_RULE [th] = th
+  | LISP_SPEC_COMPOSE_RULE (th1::th2::thms) = 
+      LISP_SPEC_COMPOSE_RULE ((SPEC_COMPOSE_RULE th1 th2)::thms)
+
+(* SEP_EXISTS tools *)
+
+(* val tm = ``(SEP_EXISTS f z. cond (z = f + 5)) s`` *)
+
+open set_sepTheory
+open wordsTheory
+
+fun SEP_EXISTS_CONV tm = let
+  val m = ``$SEP_EXISTS (P :'a -> ('b -> bool) -> bool) (x :'b -> bool)``
+  val i = match_term m tm
+  val (i,m) = match_term ((cdr o car o concl) SEP_EXISTS) ((car o car) tm)
+  val v = (fst o dest_abs o cdr o car) tm
+  val ty = (type_of o fst o dest_abs o cdr o car) tm
+  fun BETTER_ALPHA_CONV s tm = let
+    val (v,x) = dest_abs(tm)
+    in ALPHA_CONV (mk_var(s,type_of v)) tm end
+  val thi = CONV_RULE (
+              (RAND_CONV) (BETTER_ALPHA_CONV "_") THENC 
+              (RAND_CONV o ABS_CONV o ABS_CONV o RAND_CONV) 
+                (ALPHA_CONV v)) (INST_TYPE m SEP_EXISTS)
+  in (((RATOR_CONV o RATOR_CONV) (fn tm => thi))
+      THENC (RATOR_CONV BETA_CONV) THENC BETA_CONV 
+      THENC (QUANT_CONV o RATOR_CONV) BETA_CONV) tm end
+
+fun EX_TAC [] = ALL_TAC
+  | EX_TAC (x::xs) = Q.EXISTS_TAC x THEN EX_TAC xs
+
+(* print *)
+
+val _ = map Parse.hide ["r0","r1","r2","r3","r4","r5","r6","r7","r8","r9"]
+
+val one_string_IMP_string_mem = prove(
+  ``!s a c df f. one_string a s c (fun2set (f,df)) ==> string_mem s (a,f,df)``,
+  Induct
+  THEN FULL_SIMP_TAC std_ss [one_string_def,MAP,one_list_def,cond_def,
+      string_mem_def,one_STAR,IN_fun2set,GSYM AND_IMP_INTRO,fun2set_DELETE]
+  THEN ONCE_REWRITE_TAC [EQ_SYM_EQ]
+  THEN FULL_SIMP_TAC std_ss [fun2set_DELETE]
+  THEN REPEAT STRIP_TAC
+  THEN RES_TAC
+  THEN POP_ASSUM MP_TAC  
+  THEN REPEAT (POP_ASSUM (K ALL_TAC))
+  THEN Q.SPEC_TAC (`a+1w`,`b`)
+  THEN Induct_on `s`
+  THEN ASM_SIMP_TAC std_ss [string_mem_def,IN_DELETE]);
+
+val aLISP1_def = Define `
+  aLISP1 (x,l) = SEP_EXISTS x2 x3 x4 x5 x6. aLISP (x,x2,x3,x4,x5,x6,l)`;
+val pLISP1_def = Define `
+  pLISP1 (x,l) = SEP_EXISTS x2 x3 x4 x5 x6. pLISP (x,x2,x3,x4,x5,x6,l)`;
+val xLISP1_def = Define `
+  xLISP1 (x,l) = SEP_EXISTS x2 x3 x4 x5 x6. xLISP (x,x2,x3,x4,x5,x6,l)`;
+
+val aSTRING_SPACE_def = Define `
+  aSTRING_SPACE a n = SEP_EXISTS df f c. aBYTE_MEMORY df f * 
+      cond (one_space a (n + 1) c (fun2set (f,df)))`;
+val pSTRING_SPACE_def = Define `
+  pSTRING_SPACE a n = SEP_EXISTS df f c. pBYTE_MEMORY df f * 
+      cond (one_space a (n + 1) c (fun2set (f,df)))`;
+val xSTRING_SPACE_def = Define `
+  xSTRING_SPACE a n = SEP_EXISTS df f c. xBYTE_MEMORY df f * 
+      cond (one_space a (n + 1) c (fun2set (f,df)))`;
+
+val one_space_EXPAND = prove(
+  ``!n a b s. one_space a n b s = 
+              one_space a n (a + n2w n) s /\ (b = a + n2w n)``,
+  Induct  
+  THEN SIMP_TAC std_ss [one_space_def,WORD_ADD_0,cond_def,SEP_EXISTS]
+  THEN SIMP_TAC std_ss [one_STAR]    
+  THEN ONCE_ASM_REWRITE_TAC []
+  THEN SIMP_TAC std_ss [DECIDE ``SUC n = 1 + n``,GSYM word_add_n2w,WORD_ADD_ASSOC]
+  THEN METIS_TAC []);
+
+val arm_sexp2string_th = let
+  val th = arm_sexp2string_thm
+  val imp = arm_print_sexp_lemma
+  val imp = Q.INST [`r7`|->`r1`,`rest`|->`(dm,m,dg,g)`] imp
+  val imp = SIMP_RULE std_ss [] (RW1 [one_space_EXPAND] imp)
+  val imp = Q.INST [`c`|->`r1 + n2w (STRLEN (sexp2string t1) + 1)`] imp
+  val imp = RW [] imp
+  val tm = (fst o dest_imp o concl) imp
+  val th = SPEC_BOOL_FRAME_RULE th tm
+  val th = Q.INST [`r3`|->`w1`] th
+  val post = ``SEP_EXISTS r3 dg g dm m dh h. aR 3w r3 * aSTRING r3 (sexp2string t1)
+         * aBYTE_MEMORY dg g * aMEMORY dh h * aMEMORY dm m * ~aR 0w *
+         ~aR 1w * ~aR 2w * ~aR 4w * ~aR 5w * ~aR 6w * ~aR 7w
+         * ~aR 8w * ~aR 9w * aPC p * ~aS``
+  val post = subst_SPEC_PC th post 
+  val (th,goal) = SPEC_WEAKEN_RULE th post
+  val tac = 
+    SIMP_TAC std_ss [aSTRING_def]
+    THEN SIMP_TAC std_ss [SEP_CLAUSES,SEP_IMP_MOVE_COND]
+    THEN STRIP_TAC
+    THEN IMP_RES_TAC (Q.INST [`w1`|->`r3`] imp)
+    THEN FULL_SIMP_TAC (std_ss++sep_cond_ss) [arm_sexp2string_def,LET_DEF]
+    THEN SIMP_TAC std_ss [SEP_IMP_def]
+    THEN CONV_TAC (REPEATC (DEPTH_CONV SEP_EXISTS_CONV))
+    THEN REPEAT STRIP_TAC
+    THEN EX_TAC [`r1`,`dg`,`g`,`dm`,`m`,`dh`,`hi`,`df`,`fi`]
+    THEN IMP_RES_TAC one_string_IMP_string_mem
+    THEN ASM_SIMP_TAC std_ss [cond_STAR]
+    THEN FULL_SIMP_TAC std_ss [AC STAR_ASSOC STAR_COMM]
+  val th = MP th (prove(goal,tac))
+  val th = foldr (uncurry EXISTS_PRE) th [`df`,`f`,`dg`,`g`,`dm`,`m`,`dh`,`h`,`sym`]
+  val th = foldr (uncurry EXISTS_PRE) th [`t2`,`t3`,`t4`,`t5`,`t6`]
+  val th = foldr (uncurry EXISTS_PRE) th [`w1`,`w2`,`w3`,`w4`,`w5`,`w6`,`r9`]
+  val pre = ``aLISP1 (t1,l) * aR 1w r1 * aSTRING_SPACE r1 (LENGTH (sexp2string t1)) * 
+              ~aR 0w * aPC p * ~aS``
+  val (th,goal) = SPEC_STRENGTHEN_RULE th pre
+  val tac =
+    SIMP_TAC std_ss [aSTRING_SPACE_def]
+    THEN SIMP_TAC std_ss [SEP_CLAUSES,SEP_IMP_MOVE_COND]
+    THEN SIMP_TAC std_ss [aLISP1_def,aLISP_def]
+    THEN SIMP_TAC std_ss [SEP_CLAUSES,SEP_IMP_MOVE_COND]
+    THEN SIMP_TAC std_ss [SEP_IMP_def]
+    THEN CONV_TAC (REPEATC (DEPTH_CONV SEP_EXISTS_CONV))
+    THEN SIMP_TAC (std_ss++sep_cond_ss) [cond_STAR,Once one_space_EXPAND]
+    THEN NTAC 2 STRIP_TAC
+    THEN EX_TAC [`r3'`,`r4'`,`r5'`,`r6'`,`r7'`,`r8'`,`a`]
+    THEN EX_TAC [`x2`,`x3`,`x4`,`x5`,`x6`]
+    THEN EX_TAC [`df`,`f`,`dg`,`g`,`dm`,`m`,`df'`,`f'`,`s'`]
+    THEN IMP_RES_TAC imp
+    THEN ASM_SIMP_TAC std_ss [arm_sexp2string_pre_def,LET_DEF]
+    THEN SIMP_TAC (std_ss++sep_cond_ss) [Q.ISPEC `aR 4w` SEP_HIDE_def,SEP_CLAUSES]
+    THEN SIMP_TAC (std_ss++sep_cond_ss) [Q.ISPEC `aR 5w` SEP_HIDE_def,SEP_CLAUSES]
+    THEN SIMP_TAC (std_ss++sep_cond_ss) [Q.ISPEC `aR 6w` SEP_HIDE_def,SEP_CLAUSES]
+    THEN SIMP_TAC (std_ss++sep_cond_ss) [Q.ISPEC `aR 7w` SEP_HIDE_def,SEP_CLAUSES]
+    THEN SIMP_TAC (std_ss++sep_cond_ss) [Q.ISPEC `aR 8w` SEP_HIDE_def,SEP_CLAUSES]
+    THEN CONV_TAC (REPEATC (DEPTH_CONV SEP_EXISTS_CONV))
+    THEN EX_TAC [`r4'`,`r5'`,`r6'`,`r7'`,`r8'`]
+    THEN FULL_SIMP_TAC std_ss [AC STAR_ASSOC STAR_COMM]
+  val th = MP th (prove(goal,tac))
+  in th end;
+
+val ppc_sexp2string_th = let
+  val th = ppc_sexp2string_thm
+  val imp = arm_print_sexp_lemma
+  val imp = Q.INST [`r7`|->`r1`,`rest`|->`(dm,m,dg,g)`] imp
+  val imp = SIMP_RULE std_ss [] (RW1 [one_space_EXPAND] imp)
+  val imp = Q.INST [`c`|->`r1 + n2w (STRLEN (sexp2string t1) + 1)`] imp
+  val imp = RW [] imp
+  val tm = (fst o dest_imp o concl) imp
+  val th = SPEC_BOOL_FRAME_RULE th tm
+  val th = Q.INST [`r3`|->`w1`] th
+  val post = ``SEP_EXISTS r3 dg g dm m dh h. pR 3w r3 * pSTRING r3 (sexp2string t1)
+         * pBYTE_MEMORY dg g * pMEMORY dh h * pMEMORY dm m * ~pR 0w *
+         ~pR 1w * ~pR 2w * ~pR 4w * ~pR 5w * ~pR 6w * ~pR 7w
+         * ~pR 8w * ~pR 9w * pPC p * ~pS``
+  val post = subst_SPEC_PC th post 
+  val (th,goal) = SPEC_WEAKEN_RULE th post
+  val tac = 
+    SIMP_TAC std_ss [pSTRING_def]
+    THEN SIMP_TAC std_ss [SEP_CLAUSES,SEP_IMP_MOVE_COND]
+    THEN STRIP_TAC
+    THEN IMP_RES_TAC (Q.INST [`w1`|->`r3`] imp)
+    THEN FULL_SIMP_TAC (std_ss++sep_cond_ss) [ppc_sexp2string_def,LET_DEF,WORD_OR_CLAUSES]
+    THEN SIMP_TAC std_ss [SEP_IMP_def]
+    THEN CONV_TAC (REPEATC (DEPTH_CONV SEP_EXISTS_CONV))
+    THEN REPEAT STRIP_TAC
+    THEN EX_TAC [`r1`,`dg`,`g`,`dm`,`m`,`dh`,`hi`,`df`,`fi`]
+    THEN IMP_RES_TAC one_string_IMP_string_mem
+    THEN ASM_SIMP_TAC std_ss [cond_STAR]
+    THEN FULL_SIMP_TAC std_ss [AC STAR_ASSOC STAR_COMM]
+  val th = MP th (prove(goal,tac))
+  val th = foldr (uncurry EXISTS_PRE) th [`df`,`f`,`dg`,`g`,`dm`,`m`,`dh`,`h`,`sym`]
+  val th = foldr (uncurry EXISTS_PRE) th [`t2`,`t3`,`t4`,`t5`,`t6`]
+  val th = foldr (uncurry EXISTS_PRE) th [`w1`,`w2`,`w3`,`w4`,`w5`,`w6`,`r9`]
+  val pre = ``pLISP1 (t1,l) * pR 1w r1 * pSTRING_SPACE r1 (LENGTH (sexp2string t1)) * 
+              pPC p * ~pS``
+  val (th,goal) = SPEC_STRENGTHEN_RULE th pre
+  val tac =
+    SIMP_TAC std_ss [pSTRING_SPACE_def]
+    THEN SIMP_TAC std_ss [SEP_CLAUSES,SEP_IMP_MOVE_COND]
+    THEN SIMP_TAC std_ss [pLISP1_def,pLISP_def]
+    THEN SIMP_TAC std_ss [SEP_CLAUSES,SEP_IMP_MOVE_COND]
+    THEN SIMP_TAC std_ss [SEP_IMP_def]
+    THEN CONV_TAC ((REDEPTH_CONV SEP_EXISTS_CONV))
+    THEN SIMP_TAC (std_ss++sep_cond_ss) [cond_STAR,Once one_space_EXPAND]
+    THEN NTAC 2 STRIP_TAC
+    THEN EX_TAC [`r3'`,`r4'`,`r5'`,`r6'`,`r7'`,`r8'`,`a`]
+    THEN EX_TAC [`x2`,`x3`,`x4`,`x5`,`x6`]
+    THEN EX_TAC [`df`,`f`,`dg`,`g`,`dm`,`m`,`df'`,`f'`,`s'`]
+    THEN IMP_RES_TAC imp
+    THEN ASM_SIMP_TAC std_ss [ppc_sexp2string_pre_def,LET_DEF,WORD_OR_CLAUSES]
+    THEN SIMP_TAC (std_ss++sep_cond_ss) [Q.ISPEC `pR 4w` SEP_HIDE_def,SEP_CLAUSES]
+    THEN SIMP_TAC (std_ss++sep_cond_ss) [Q.ISPEC `pR 5w` SEP_HIDE_def,SEP_CLAUSES]
+    THEN SIMP_TAC (std_ss++sep_cond_ss) [Q.ISPEC `pR 6w` SEP_HIDE_def,SEP_CLAUSES]
+    THEN SIMP_TAC (std_ss++sep_cond_ss) [Q.ISPEC `pR 7w` SEP_HIDE_def,SEP_CLAUSES]
+    THEN SIMP_TAC (std_ss++sep_cond_ss) [Q.ISPEC `pR 8w` SEP_HIDE_def,SEP_CLAUSES]
+    THEN CONV_TAC (REPEATC (DEPTH_CONV SEP_EXISTS_CONV))
+    THEN EX_TAC [`r4'`,`r5'`,`r6'`,`r7'`,`r8'`]
+    THEN FULL_SIMP_TAC std_ss [AC STAR_ASSOC STAR_COMM]
+  val th = MP th (prove(goal,tac))
+  in th end;
+
+val xSTACK_def = Define `
+  (xSTACK a [] = cond (ALIGNED a)) /\ 
+  (xSTACK a (w::ws) = xM a w * xSTACK (a + 4w) ws)`;
+
+val xSTACK_PUSH_EDI = let
+  val (th,t_def) = decompilerLib.decompile 
+    prog_x86Lib.x86_tools "test" [QUOTE (x86_encodeLib.x86_encode "push edi")]
+  val th = SIMP_RULE std_ss [t_def,LET_DEF] th
+  val th = Q.INST [`df`|->`{esp - 4w}`,`f`|->`\x.w`] th
+  val th = SPEC_BOOL_FRAME_RULE th ``ALIGNED esp`` 
+  val post = ``xSTACK (esp-4w) [edi] * xR EDI edi * xR ESP (esp - 0x4w) * xPC (p + 0x1w)``    
+  val (th,goal) = SPEC_WEAKEN_RULE th post
+  val tac = 
+    SIMP_TAC std_ss [SEP_IMP_MOVE_COND,xSTACK_def,prog_x86Theory.xM_THM,
+      ALIGNED,SEP_CLAUSES] THEN SIMP_TAC (std_ss++star_ss) [SEP_IMP_REFL]  
+  val th = MP th (prove(goal,tac))
+  val pre = ``xSTACK (esp-4w) [w] * xR EDI edi * xR ESP esp * xPC p``    
+  val (th,goal) = SPEC_STRENGTHEN_RULE th pre
+  val tac = 
+    SIMP_TAC (std_ss++sep_cond_ss) [SEP_IMP_MOVE_COND,xSTACK_def,prog_x86Theory.xM_THM,
+      ALIGNED,SEP_CLAUSES,SEP_IMP_REFL,IN_INSERT,NOT_IN_EMPTY] 
+    THEN SIMP_TAC (std_ss++star_ss) [ALIGNED_INTRO,ALIGNED,SEP_CLAUSES,SEP_IMP_REFL]  
+  val th = MP th (prove(goal,tac))
+  in th end;
+ 
+val xSTACK_MOVE_EDI = let
+  val (th,t_def) = decompilerLib.decompile 
+    prog_x86Lib.x86_tools "test" [QUOTE (x86_encodeLib.x86_encode "mov edi, [esp]")]
+  val th = SIMP_RULE std_ss [t_def,LET_DEF] th
+  val th = Q.INST [`df`|->`{esp}`,`f`|->`\x.w`] th
+  val th = SPEC_BOOL_FRAME_RULE th ``ALIGNED esp`` 
+  val post = ``xSTACK esp [w] * xR EDI w * xR ESP esp * xPC (p + 0x3w)``    
+  val (th,goal) = SPEC_WEAKEN_RULE th post
+  val tac = 
+    SIMP_TAC std_ss [SEP_IMP_MOVE_COND,xSTACK_def,prog_x86Theory.xM_THM,
+      ALIGNED,SEP_CLAUSES] THEN SIMP_TAC (std_ss++star_ss) [SEP_IMP_REFL]  
+  val th = MP th (prove(goal,tac))
+  val pre = ``xSTACK esp [w] * ~xR EDI * xR ESP esp * xPC p``    
+  val (th,goal) = SPEC_STRENGTHEN_RULE th pre
+  val tac = 
+    SIMP_TAC (std_ss++sep_cond_ss) [SEP_IMP_MOVE_COND,xSTACK_def,prog_x86Theory.xM_THM,
+      ALIGNED,SEP_CLAUSES,SEP_IMP_REFL,IN_INSERT,NOT_IN_EMPTY] 
+    THEN SIMP_TAC (std_ss++star_ss) [ALIGNED_INTRO,ALIGNED,SEP_CLAUSES,SEP_IMP_REFL]  
+  val th = MP th (prove(goal,tac))
+  in th end;
+
+val xSTACK_POP_EDI = let
+  val (th,t_def) = decompilerLib.decompile 
+    prog_x86Lib.x86_tools "test" [QUOTE (x86_encodeLib.x86_encode "pop edi")]
+  val th = SIMP_RULE std_ss [t_def,LET_DEF] th
+  val th = Q.INST [`df`|->`{esp}`,`f`|->`\x.w`] th
+  val th = SPEC_BOOL_FRAME_RULE th ``ALIGNED esp`` 
+  val post = ``xSTACK esp [w] * xR EDI w * xR ESP (esp+4w) * xPC (p + 0x1w)``    
+  val (th,goal) = SPEC_WEAKEN_RULE th post
+  val tac = 
+    SIMP_TAC std_ss [SEP_IMP_MOVE_COND,xSTACK_def,prog_x86Theory.xM_THM,
+      ALIGNED,SEP_CLAUSES] THEN SIMP_TAC (std_ss++star_ss) [SEP_IMP_REFL]  
+  val th = MP th (prove(goal,tac))
+  val pre = ``xSTACK esp [w] * ~xR EDI * xR ESP esp * xPC p``    
+  val (th,goal) = SPEC_STRENGTHEN_RULE th pre
+  val tac = 
+    SIMP_TAC (std_ss++sep_cond_ss) [SEP_IMP_MOVE_COND,xSTACK_def,prog_x86Theory.xM_THM,
+      ALIGNED,SEP_CLAUSES,SEP_IMP_REFL,IN_INSERT,NOT_IN_EMPTY] 
+    THEN SIMP_TAC (std_ss++star_ss) [ALIGNED_INTRO,ALIGNED,SEP_CLAUSES,SEP_IMP_REFL]  
+  val th = MP th (prove(goal,tac))
+  in th end;
+
+val x86_sexp2string_th = let
+  val th = SPEC_COMPOSE_RULE xSTACK_MOVE_EDI x86_sexp2string_thm
+  val post = ``(let (eax,ecx,edi,esi,ebp,dh,h,df,f,dm,m,dg,g) =
+             arm_print_sexp (eax,w,ebp,dh,h,df,f,dm,m,dg,g)
+       in
+         xBYTE_MEMORY df f * xBYTE_MEMORY dg g * xMEMORY dh h *
+         xMEMORY dm m * xR EAX eax * xR EBP ebp * ~xR EBX * xR ECX ecx *
+         ~xR EDX * xR ESI esi * ~xS) *
+      (~xR EDI * xSTACK esp [w] * xR ESP esp * xPC p)``
+  val post = subst_SPEC_PC th post
+  val (th,goal) = SPEC_WEAKEN_RULE th post
+  val tac = 
+    SIMP_TAC std_ss [LET_DEF]
+    THEN CONV_TAC (DEPTH_CONV FORCE_PBETA_CONV)
+    THEN SIMP_TAC (std_ss++sep_cond_ss) [Q.ISPEC `xR EDI` SEP_HIDE_def,SEP_CLAUSES]
+    THEN SIMP_TAC std_ss [SEP_IMP_def]
+    THEN CONV_TAC (REPEATC (DEPTH_CONV SEP_EXISTS_CONV))
+    THEN REPEAT STRIP_TAC
+    THEN Q.EXISTS_TAC `(FST
+        (SND (SND (arm_print_sexp (eax,w,ebp,dh,h,df,f,dm,m,dg,g)))))`
+    THEN FULL_SIMP_TAC std_ss [AC STAR_COMM STAR_ASSOC]
+  val th = MP th (prove(goal,tac))
+  val th = SPEC_COMPOSE_RULE th xSTACK_POP_EDI  
+  val th = RW [] (DISCH_ALL th)
+  val imp = arm_print_sexp_lemma
+  val imp = Q.INST [`r7`|->`r1`,`rest`|->`(dm,m,dg,g)`] imp
+  val imp = SIMP_RULE std_ss [] (RW1 [one_space_EXPAND] imp)
+  val imp = Q.INST [`c`|->`r1 + n2w (STRLEN (sexp2string t1) + 1)`] imp
+  val imp = RW [] imp
+  val tm = (fst o dest_imp o concl) imp
+  val th = SPEC_BOOL_FRAME_RULE th tm
+  val th = Q.INST [`eax`|->`w1`,`ebp`|->`r9`,`r1`|->`w`] th
+  val post = ``SEP_EXISTS edi dg g dm m dh h. xR EDI edi * xSTRING edi (sexp2string t1)
+         * xBYTE_MEMORY dg g * xMEMORY dh h * xMEMORY dm m * 
+         ~xR EAX * ~xR EBP * ~xR EBX * ~xR ECX * ~xR EDX * ~xR ESI
+         * xPC p * ~xS * xSTACK esp [w] * xR ESP (esp + 0x4w)``
+  val post = subst_SPEC_PC th post 
+  val (th,goal) = SPEC_WEAKEN_RULE th post
+  val tac = 
+    SIMP_TAC std_ss [xSTRING_def]
+    THEN SIMP_TAC std_ss [SEP_CLAUSES,SEP_IMP_MOVE_COND]
+    THEN STRIP_TAC
+    THEN IMP_RES_TAC imp
+    THEN FULL_SIMP_TAC (std_ss++sep_cond_ss) [LET_DEF,WORD_OR_CLAUSES]
+    THEN SIMP_TAC std_ss [SEP_IMP_def]
+    THEN CONV_TAC (REPEATC (DEPTH_CONV SEP_EXISTS_CONV))
+    THEN REPEAT STRIP_TAC
+    THEN EX_TAC [`w`,`dg`,`g`,`dm`,`m`,`dh`,`hi`,`df`,`fi`]
+    THEN IMP_RES_TAC one_string_IMP_string_mem
+    THEN ASM_SIMP_TAC std_ss [cond_STAR]
+    THEN SIMP_TAC (std_ss++sep_cond_ss) [Q.ISPEC `xR ECX` SEP_HIDE_def,SEP_CLAUSES]
+    THEN CONV_TAC (REPEATC (DEPTH_CONV SEP_EXISTS_CONV))
+    THEN EX_TAC [`r4i`]
+    THEN SIMP_TAC (std_ss++sep_cond_ss) [Q.ISPEC `xR EAX` SEP_HIDE_def,SEP_CLAUSES]
+    THEN CONV_TAC (REPEATC (DEPTH_CONV SEP_EXISTS_CONV))
+    THEN EX_TAC [`w`]
+    THEN SIMP_TAC (std_ss++sep_cond_ss) [Q.ISPEC `xR EBP` SEP_HIDE_def,SEP_CLAUSES]
+    THEN CONV_TAC (REPEATC (DEPTH_CONV SEP_EXISTS_CONV))
+    THEN EX_TAC [`r9`]
+    THEN SIMP_TAC (std_ss++sep_cond_ss) [Q.ISPEC `xR ESI` SEP_HIDE_def,SEP_CLAUSES]
+    THEN CONV_TAC (REPEATC (DEPTH_CONV SEP_EXISTS_CONV))
+    THEN EX_TAC [`r8i`]
+    THEN FULL_SIMP_TAC std_ss [AC STAR_ASSOC STAR_COMM]
+  val th = MP th (prove(goal,tac))
+  val th = foldr (uncurry EXISTS_PRE) th [`df`,`f`,`dg`,`g`,`dm`,`m`,`dh`,`h`,`sym`]
+  val th = foldr (uncurry EXISTS_PRE) th [`t2`,`t3`,`t4`,`t5`,`t6`]
+  val th = foldr (uncurry EXISTS_PRE) th [`w1`,`w2`,`w3`,`w4`,`w5`,`w6`,`r9`]
+  val pre = ``xLISP1 (t1,l) * xSTRING_SPACE w (LENGTH (sexp2string t1)) * 
+              xPC p * ~xS * xSTACK esp [w] * xR ESP esp``
+  val (th,goal) = SPEC_STRENGTHEN_RULE th pre
+  val tac =
+    SIMP_TAC std_ss [xSTRING_SPACE_def]
+    THEN SIMP_TAC std_ss [SEP_CLAUSES,SEP_IMP_MOVE_COND]
+    THEN SIMP_TAC std_ss [xLISP1_def,xLISP_def]
+    THEN SIMP_TAC std_ss [SEP_CLAUSES,SEP_IMP_MOVE_COND]
+    THEN SIMP_TAC std_ss [SEP_IMP_def]
+    THEN CONV_TAC ((REDEPTH_CONV SEP_EXISTS_CONV))
+    THEN SIMP_TAC (std_ss++sep_cond_ss) [cond_STAR,Once one_space_EXPAND]
+    THEN NTAC 2 STRIP_TAC
+    THEN EX_TAC [`r3'`,`r4'`,`r5'`,`r6'`,`r7'`,`r8'`,`a`]
+    THEN EX_TAC [`x2`,`x3`,`x4`,`x5`,`x6`]
+    THEN EX_TAC [`df`,`f`,`dg`,`g`,`dm`,`m`,`df'`,`f'`,`s'`]
+    THEN IMP_RES_TAC imp
+    THEN ASM_SIMP_TAC std_ss [LET_DEF,WORD_OR_CLAUSES]
+    THEN SIMP_TAC (std_ss++sep_cond_ss) [Q.ISPEC `xR ESI` SEP_HIDE_def,SEP_CLAUSES]
+    THEN CONV_TAC (REPEATC (DEPTH_CONV SEP_EXISTS_CONV))
+    THEN EX_TAC [`r8'`]
+    THEN SIMP_TAC (std_ss++sep_cond_ss) [Q.ISPEC `xR EDI` SEP_HIDE_def,SEP_CLAUSES]
+    THEN CONV_TAC (REPEATC (DEPTH_CONV SEP_EXISTS_CONV))
+    THEN EX_TAC [`r7'`]
+    THEN SIMP_TAC (std_ss++sep_cond_ss) [Q.ISPEC `xR EBX` SEP_HIDE_def,SEP_CLAUSES]
+    THEN CONV_TAC (REPEATC (DEPTH_CONV SEP_EXISTS_CONV))
+    THEN EX_TAC [`r6'`]
+    THEN SIMP_TAC (std_ss++sep_cond_ss) [Q.ISPEC `xR EDX` SEP_HIDE_def,SEP_CLAUSES]
+    THEN CONV_TAC (REPEATC (DEPTH_CONV SEP_EXISTS_CONV))
+    THEN EX_TAC [`r5'`]
+    THEN SIMP_TAC (std_ss++sep_cond_ss) [Q.ISPEC `xR ECX` SEP_HIDE_def,SEP_CLAUSES]
+    THEN CONV_TAC (REPEATC (DEPTH_CONV SEP_EXISTS_CONV))
+    THEN EX_TAC [`r4'`]
+    THEN FULL_SIMP_TAC std_ss [AC STAR_ASSOC STAR_COMM]
+  val th = MP th (prove(goal,tac))
+  in th end;
+
+val R_ev_thm = let
+  val rw = RW [] (MATCH_MP SET_TO_LIST_THM FINITE_EMPTY)
+  val thi = Q.SPECL [`s`,`FEMPTY`,`t`,`l`] LISP_EVAL_CORRECT
+  val thi = CONJ thi (Q.SPECL [`s`,`FEMPTY`,`t`,`l`] LISP_EVAL_LIMIT_CORRECT)
+  val thi = SIMP_RULE std_ss [rw,fmap2list_def,FDOM_FEMPTY,MAP,alist2sexp_def,list2sexp_def,LISP_EVAL_def] thi
+  in thi end;
+
+fun auto_prove th post = let
+  val th = Q.INST [`x`|->`Sym "nil"`] th
+  val th = Q.INST [`y`|->`Sym "nil"`] th
+  val th = Q.INST [`z`|->`Sym "nil"`] th
+  val th = Q.INST [`stack`|->`Sym "nil"`] th
+  val th = Q.INST [`alist`|->`Sym "nil"`] th
+  val post = subst_SPEC_PC th post 
+  val th = SPEC_BOOL_FRAME_RULE th ``R_ev (s,FEMPTY) s2 /\ (exp = term2sexp s)``
+  val (th,goal) = SPEC_WEAKEN_RULE th post
+  val tac = 
+    SIMP_TAC std_ss [LISP_EVAL_def,aLISP1_def,pLISP1_def,xLISP1_def]  
+    THEN `?exp2 x2 y2 z2 stack2 alist2 l2. 
+       lisp_eval (exp,Sym "nil",Sym "nil",Sym "nil",Sym "nil",Sym "nil",l) = 
+       (exp2,x2,y2,z2,stack2,alist2,l2)` by METIS_TAC [pairTheory.PAIR]
+    THEN ASM_SIMP_TAC std_ss [LET_DEF,SEP_IMP_def,cond_STAR]
+    THEN SIMP_TAC std_ss [SEP_CLAUSES]    
+    THEN CONV_TAC (REPEATC (DEPTH_CONV SEP_EXISTS_CONV))
+    THEN REPEAT STRIP_TAC
+    THEN EX_TAC [`x2`,`y2`,`z2`,`stack2`,`alist2`]
+    THEN FULL_SIMP_TAC std_ss []
+    THEN MP_TAC (Q.INST [`t`|->`s2`] R_ev_thm)
+    THEN ASM_SIMP_TAC std_ss []
+    THEN REPEAT STRIP_TAC
+    THEN FULL_SIMP_TAC std_ss []
+  val th = MP th (prove(goal,tac))
+  in th end;  
+
+val arm_th = auto_prove SPEC_lisp_eval_arm_thm
+  ``aLISP1 (sexpression2sexp s2,l) * aPC p * ~aS``
+
+val ppc_th = auto_prove SPEC_lisp_eval_ppc_thm
+  ``pLISP1 (sexpression2sexp s2,l) * pPC p * ~pS``
+
+val x86_th = auto_prove SPEC_lisp_eval_x86_thm
+  ``xLISP1 (sexpression2sexp s2,l) * xPC p * ~xS``
+
+val _ = codegen_x86Lib.set_x86_regs 
+  [(3,"eax"),(4,"ecx"),(5,"edx"),(6,"ebx"),(7,"edi"),(8,"esi")]
+
+val (th1,th2,th3) = compilerLib.compile_all `` 
+  add32 (r5:word32) = let r5 = r5 + 32w in r5``;
+
+val setup_code = 
+  map (fn (s,th) => (s,SIMP_RULE std_ss [th2,th3,LET_DEF,SEP_CLAUSES] th)) th1
+
+fun find_thm t [] = hd []
+  | find_thm t ((s,th)::xs) = if t = s then th else find_thm t xs
+
+val arm_eval_th = LISP_SPEC_COMPOSE_RULE 
+  [find_thm "arm" setup_code,
+   arm_string2sexp_arm_thm,
+   arm_th,
+   arm_sexp2string_th]
+
+val ppc_eval_th = LISP_SPEC_COMPOSE_RULE 
+  [find_thm "ppc" setup_code,
+   arm_string2sexp_ppc_thm,
+   ppc_th,
+   ppc_sexp2string_th]
+
+val x86_eval_th = LISP_SPEC_COMPOSE_RULE 
+  [find_thm "x86" setup_code,
+   xSTACK_PUSH_EDI,
+   arm_string2sexp_x86_thm,
+   x86_th,
+   Q.INST [`w`|->`edi`,`esp`|->`esp-4w`] x86_sexp2string_th]
+
+
+val _ = save_thm("arm_eval_th",arm_eval_th);
+val _ = save_thm("ppc_eval_th",ppc_eval_th);
+val _ = save_thm("x86_eval_th",x86_eval_th);
+
+open export_codeLib;
+
+val _ = write_code_to_file "arm_eval.s" arm_eval_th
+val _ = write_code_to_file "ppc_eval.s" ppc_eval_th
+val _ = write_code_to_file "x86_eval.s" x86_eval_th
+
+val _ = export_theory();
